subtyping properties

spectec/isabelle_type_safety_proof/Subtyping.thy
@@ -2,13 +2,17 @@ section \<open>Subtyping\<close>
 
 theory Subtyping imports reference_isabelle_output_wasm2 begin
 
+(*
+this is 7187 Valtype_sub:
+
 definition t_subtyping :: "[valtype, valtype] \<Rightarrow> bool" ("_ '<t: _" 60) where
   "t_subtyping t1 t2 = (t1 = BOT \<or> t1 = t2)"
+*)
 
 definition t_list_subtyping :: "[resulttype, resulttype] \<Rightarrow> bool" ("_ '<ts: _" 60) where
   "t_list_subtyping t1 t2 =
     (case (t1, t2) of
-      (mk_list t1s, mk_list t2s) \<Rightarrow> list_all2 t_subtyping t1s t2s)"
+      (mk_list t1s, mk_list t2s) \<Rightarrow> list_all2 Valtype_sub t1s t2s)"
 
 definition instr_subtyping :: "[functype, functype] \<Rightarrow> bool" ("_ '<ti: _" 60) where
   "instr_subtyping tf1 tf2  \<equiv> 
@@ -16,9 +20,54 @@ definition instr_subtyping :: "[functype, functype] \<Rightarrow> bool" ("_ '<ti
  (mk_functype (mk_list dom1) (mk_list ran1), mk_functype (mk_list dom2) (mk_list ran2)) \<Rightarrow> \<exists> ts ts' tf1_dom_sub tf1_ran_sub.
     dom2 = ts@tf1_dom_sub
   \<and> ran2 = ts'@tf1_ran_sub
-  \<and> t_list_subtyping (mk_list ts) (mk_list ts')
-  \<and> t_list_subtyping (mk_list tf1_dom_sub)  (mk_list dom1)
-  \<and> t_list_subtyping (mk_list ran1) (mk_list tf1_ran_sub)
+  \<and> Resulttype_sub (mk_list ts) (mk_list ts')
+  \<and> Resulttype_sub (mk_list tf1_dom_sub)  (mk_list dom1)
+  \<and> Resulttype_sub (mk_list ran1) (mk_list tf1_ran_sub)
 )"
+
+lemma Resulttype_sub_t_list_subtyping:
+  "Resulttype_sub rt1 rt2 \<longleftrightarrow> t_list_subtyping rt1 rt2"
+  apply auto
+  subgoal
+    apply (induction rule: Resulttype_sub.induct)
+    using t_list_subtyping_def by auto
+  subgoal
+    unfolding t_list_subtyping_def
+    apply (auto split: prod.splits)
+    by (metis list_all2_lengthD mk_Resulttype_sub res_list.case res_list.exhaust)
+  done
+
+lemma Resulttype_sub_empty:
+  "Resulttype_sub (mk_list []) (mk_list [])"
+  by (auto simp add: Resulttype_sub.simps)
+
+lemma instr_subtyping_sub_rule:
+  assumes
+    "Resulttype_sub ts1' ts1"
+    "Resulttype_sub ts2 ts2'"
+  shows
+    "(mk_functype ts1 ts2) <ti: (mk_functype ts1' ts2')"
+  using assms Resulttype_sub_t_list_subtyping unfolding instr_subtyping_def
+  apply (auto split: res_list.splits)
+  sorry
+
+lemma instr_subtyping_frame_rule:
+    "(mk_functype (mk_list ts1) (mk_list ts2)) <ti: (mk_functype (mk_list (ts@ts1)) (mk_list (ts@ts2)))"
+  using assms Resulttype_sub_t_list_subtyping unfolding instr_subtyping_def
+  apply (auto split: res_list.splits)
+  sorry
+
+
+lemma instr_subtyping_trans:
+  assumes
+    "tf1 <ti: tf2"
+    "tf2 <ti: tf3"
+  shows
+    "tf1 <ti: tf3"
+  sorry
+
+
+
+
 
 end
