spectec/isabelle_type_safety_proof/Properties_Aux.thy
@@ -1,0 +1,24 @@
+theory Properties_Aux
+	imports Main reference_isabelle_output_wasm2 Subtyping
+begin
+
+lemma b_e_type_empty1[dest]:
+  assumes "Instrs_ok C [] ft"
+          "ft = (mk_functype (mk_list ts) (mk_list ts'))"
+  shows   "instr_subtyping (mk_functype (mk_list []) (mk_list [])) (mk_functype (mk_list ts) (mk_list ts'))"
+  using assms
+  apply (induction "[] :: (instr list)" "ft" arbitrary: ts ts' rule: Instr_ok_Instrs_ok.inducts(2))
+                      apply auto
+  subgoal
+    unfolding instr_subtyping_def
+    using Resulttype_sub_empty
+    by (auto split: res_list.splits)
+  subgoal for C t_1_lst t_2_lst t'_2_lst ts
+    using instr_subtyping_trans instr_subtyping_sub_rule
+    by auto
+  subgoal
+    using instr_subtyping_trans instr_subtyping_frame_rule
+    by auto
+  done
+
+end
